Shallow_Micro_C/C_Arithmetic_Rules.thy
@@ -278,6 +278,201 @@ lemma wp_c_unsigned_eqI [micro_rust_wp_intros]:
   shows \<open>\<phi> \<longlongrightarrow> \<W>\<P> \<Gamma> (c_unsigned_eq a b) \<psi> \<rho> \<theta>\<close>
   using assms by (simp add: c_unsigned_eq_def wp_literalI)
 
+subsection \<open>Signed Bitwise Operations\<close>
+
+lemma wp_c_signed_and [micro_rust_wp_simps]:
+  fixes a b :: \<open>'l::{len} sword\<close>
+  assumes \<open>\<And>r. ucincl (\<psi> r)\<close>
+  shows \<open>\<W>\<P> \<Gamma> (c_signed_and a b) \<psi> \<rho> \<theta> = \<psi> (a AND b)\<close>
+  using assms by (simp add: c_signed_and_def micro_rust_wp_simps)
+
+lemma wp_c_signed_andI [micro_rust_wp_intros]:
+  fixes a b :: \<open>'l::{len} sword\<close>
+  assumes \<open>\<phi> \<longlongrightarrow> \<psi> (a AND b) \<star> \<top>\<close>
+  shows \<open>\<phi> \<longlongrightarrow> \<W>\<P> \<Gamma> (c_signed_and a b) \<psi> \<rho> \<theta>\<close>
+  using assms by (simp add: c_signed_and_def wp_literalI)
+
+lemma wp_c_signed_or [micro_rust_wp_simps]:
+  fixes a b :: \<open>'l::{len} sword\<close>
+  assumes \<open>\<And>r. ucincl (\<psi> r)\<close>
+  shows \<open>\<W>\<P> \<Gamma> (c_signed_or a b) \<psi> \<rho> \<theta> = \<psi> (a OR b)\<close>
+  using assms by (simp add: c_signed_or_def micro_rust_wp_simps)
+
+lemma wp_c_signed_orI [micro_rust_wp_intros]:
+  fixes a b :: \<open>'l::{len} sword\<close>
+  assumes \<open>\<phi> \<longlongrightarrow> \<psi> (a OR b) \<star> \<top>\<close>
+  shows \<open>\<phi> \<longlongrightarrow> \<W>\<P> \<Gamma> (c_signed_or a b) \<psi> \<rho> \<theta>\<close>
+  using assms by (simp add: c_signed_or_def wp_literalI)
+
+lemma wp_c_signed_xor [micro_rust_wp_simps]:
+  fixes a b :: \<open>'l::{len} sword\<close>
+  assumes \<open>\<And>r. ucincl (\<psi> r)\<close>
+  shows \<open>\<W>\<P> \<Gamma> (c_signed_xor a b) \<psi> \<rho> \<theta> = \<psi> (a XOR b)\<close>
+  using assms by (simp add: c_signed_xor_def micro_rust_wp_simps)
+
+lemma wp_c_signed_xorI [micro_rust_wp_intros]:
+  fixes a b :: \<open>'l::{len} sword\<close>
+  assumes \<open>\<phi> \<longlongrightarrow> \<psi> (a XOR b) \<star> \<top>\<close>
+  shows \<open>\<phi> \<longlongrightarrow> \<W>\<P> \<Gamma> (c_signed_xor a b) \<psi> \<rho> \<theta>\<close>
+  using assms by (simp add: c_signed_xor_def wp_literalI)
+
+lemma wp_c_signed_not [micro_rust_wp_simps]:
+  fixes a :: \<open>'l::{len} sword\<close>
+  assumes \<open>\<And>r. ucincl (\<psi> r)\<close>
+  shows \<open>\<W>\<P> \<Gamma> (c_signed_not a) \<psi> \<rho> \<theta> = \<psi> (NOT a)\<close>
+  using assms by (simp add: c_signed_not_def micro_rust_wp_simps)
+
+lemma wp_c_signed_notI [micro_rust_wp_intros]:
+  fixes a :: \<open>'l::{len} sword\<close>
+  assumes \<open>\<phi> \<longlongrightarrow> \<psi> (NOT a) \<star> \<top>\<close>
+  shows \<open>\<phi> \<longlongrightarrow> \<W>\<P> \<Gamma> (c_signed_not a) \<psi> \<rho> \<theta>\<close>
+  using assms by (simp add: c_signed_not_def wp_literalI)
+
+subsection \<open>Unsigned Bitwise Operations\<close>
+
+lemma wp_c_unsigned_and [micro_rust_wp_simps]:
+  fixes a b :: \<open>'l::{len} word\<close>
+  assumes \<open>\<And>r. ucincl (\<psi> r)\<close>
+  shows \<open>\<W>\<P> \<Gamma> (c_unsigned_and a b) \<psi> \<rho> \<theta> = \<psi> (a AND b)\<close>
+  using assms by (simp add: c_unsigned_and_def micro_rust_wp_simps)
+
+lemma wp_c_unsigned_andI [micro_rust_wp_intros]:
+  fixes a b :: \<open>'l::{len} word\<close>
+  assumes \<open>\<phi> \<longlongrightarrow> \<psi> (a AND b) \<star> \<top>\<close>
+  shows \<open>\<phi> \<longlongrightarrow> \<W>\<P> \<Gamma> (c_unsigned_and a b) \<psi> \<rho> \<theta>\<close>
+  using assms by (simp add: c_unsigned_and_def wp_literalI)
+
+lemma wp_c_unsigned_or [micro_rust_wp_simps]:
+  fixes a b :: \<open>'l::{len} word\<close>
+  assumes \<open>\<And>r. ucincl (\<psi> r)\<close>
+  shows \<open>\<W>\<P> \<Gamma> (c_unsigned_or a b) \<psi> \<rho> \<theta> = \<psi> (a OR b)\<close>
+  using assms by (simp add: c_unsigned_or_def micro_rust_wp_simps)
+
+lemma wp_c_unsigned_orI [micro_rust_wp_intros]:
+  fixes a b :: \<open>'l::{len} word\<close>
+  assumes \<open>\<phi> \<longlongrightarrow> \<psi> (a OR b) \<star> \<top>\<close>
+  shows \<open>\<phi> \<longlongrightarrow> \<W>\<P> \<Gamma> (c_unsigned_or a b) \<psi> \<rho> \<theta>\<close>
+  using assms by (simp add: c_unsigned_or_def wp_literalI)
+
+lemma wp_c_unsigned_xor [micro_rust_wp_simps]:
+  fixes a b :: \<open>'l::{len} word\<close>
+  assumes \<open>\<And>r. ucincl (\<psi> r)\<close>
+  shows \<open>\<W>\<P> \<Gamma> (c_unsigned_xor a b) \<psi> \<rho> \<theta> = \<psi> (a XOR b)\<close>
+  using assms by (simp add: c_unsigned_xor_def micro_rust_wp_simps)
+
+lemma wp_c_unsigned_xorI [micro_rust_wp_intros]:
+  fixes a b :: \<open>'l::{len} word\<close>
+  assumes \<open>\<phi> \<longlongrightarrow> \<psi> (a XOR b) \<star> \<top>\<close>
+  shows \<open>\<phi> \<longlongrightarrow> \<W>\<P> \<Gamma> (c_unsigned_xor a b) \<psi> \<rho> \<theta>\<close>
+  using assms by (simp add: c_unsigned_xor_def wp_literalI)
+
+lemma wp_c_unsigned_not [micro_rust_wp_simps]:
+  fixes a :: \<open>'l::{len} word\<close>
+  assumes \<open>\<And>r. ucincl (\<psi> r)\<close>
+  shows \<open>\<W>\<P> \<Gamma> (c_unsigned_not a) \<psi> \<rho> \<theta> = \<psi> (NOT a)\<close>
+  using assms by (simp add: c_unsigned_not_def micro_rust_wp_simps)
+
+lemma wp_c_unsigned_notI [micro_rust_wp_intros]:
+  fixes a :: \<open>'l::{len} word\<close>
+  assumes \<open>\<phi> \<longlongrightarrow> \<psi> (NOT a) \<star> \<top>\<close>
+  shows \<open>\<phi> \<longlongrightarrow> \<W>\<P> \<Gamma> (c_unsigned_not a) \<psi> \<rho> \<theta>\<close>
+  using assms by (simp add: c_unsigned_not_def wp_literalI)
+
+subsection \<open>Unsigned Shift Operations\<close>
+
+lemma wp_c_unsigned_shl [micro_rust_wp_simps]:
+  fixes a b :: \<open>'l::{len} word\<close>
+  assumes \<open>\<And>r. ucincl (\<psi> r)\<close>
+  shows \<open>\<W>\<P> \<Gamma> (c_unsigned_shl a b) \<psi> \<rho> \<theta> =
+    (if unat b < LENGTH('l)
+     then \<psi> (push_bit (unat b) a)
+     else \<theta> (CustomAbort ShiftOutOfRange) \<star> UNIV)\<close>
+  using assms
+  by (simp add: c_unsigned_shl_def c_shift_out_of_range_def c_abort_def micro_rust_wp_simps)
+
+lemma wp_c_unsigned_shlI [micro_rust_wp_intros]:
+  fixes a b :: \<open>'l::{len} word\<close>
+  assumes \<open>unat b < LENGTH('l)\<close>
+      and \<open>\<phi> \<longlongrightarrow> \<psi> (push_bit (unat b) a) \<star> \<top>\<close>
+  shows \<open>\<phi> \<longlongrightarrow> \<W>\<P> \<Gamma> (c_unsigned_shl a b) \<psi> \<rho> \<theta>\<close>
+proof -
+  from assms(1) have eq: \<open>c_unsigned_shl a b = literal (push_bit (unat b) a)\<close>
+    by (simp add: c_unsigned_shl_def)
+  show ?thesis unfolding eq using assms(2) by (rule wp_literalI)
+qed
+
+lemma wp_c_unsigned_shr [micro_rust_wp_simps]:
+  fixes a b :: \<open>'l::{len} word\<close>
+  assumes \<open>\<And>r. ucincl (\<psi> r)\<close>
+  shows \<open>\<W>\<P> \<Gamma> (c_unsigned_shr a b) \<psi> \<rho> \<theta> =
+    (if unat b < LENGTH('l)
+     then \<psi> (drop_bit (unat b) a)
+     else \<theta> (CustomAbort ShiftOutOfRange) \<star> UNIV)\<close>
+  using assms
+  by (simp add: c_unsigned_shr_def c_shift_out_of_range_def c_abort_def micro_rust_wp_simps)
+
+lemma wp_c_unsigned_shrI [micro_rust_wp_intros]:
+  fixes a b :: \<open>'l::{len} word\<close>
+  assumes \<open>unat b < LENGTH('l)\<close>
+      and \<open>\<phi> \<longlongrightarrow> \<psi> (drop_bit (unat b) a) \<star> \<top>\<close>
+  shows \<open>\<phi> \<longlongrightarrow> \<W>\<P> \<Gamma> (c_unsigned_shr a b) \<psi> \<rho> \<theta>\<close>
+proof -
+  from assms(1) have eq: \<open>c_unsigned_shr a b = literal (drop_bit (unat b) a)\<close>
+    by (simp add: c_unsigned_shr_def)
+  show ?thesis unfolding eq using assms(2) by (rule wp_literalI)
+qed
+
+subsection \<open>Signed Shift Operations\<close>
+
+lemma wp_c_signed_shl [micro_rust_wp_simps]:
+  fixes a b :: \<open>'l::{len} sword\<close>
+  assumes \<open>\<And>r. ucincl (\<psi> r)\<close>
+  shows \<open>\<W>\<P> \<Gamma> (c_signed_shl a b) \<psi> \<rho> \<theta> =
+    (if unat b \<ge> LENGTH('l) then \<theta> (CustomAbort ShiftOutOfRange) \<star> UNIV
+     else let result_int = sint a * 2 ^ unat b in
+       if sint a < 0 \<or> \<not> c_signed_in_range result_int LENGTH('l) then
+         \<theta> (CustomAbort SignedOverflow) \<star> UNIV
+       else \<psi> (word_of_int result_int))\<close>
+  using assms
+  by (simp add: c_signed_shl_def c_shift_out_of_range_def c_signed_overflow_def
+                c_abort_def Let_def micro_rust_wp_simps)
+
+lemma wp_c_signed_shlI [micro_rust_wp_intros]:
+  fixes a b :: \<open>'l::{len} sword\<close>
+  assumes \<open>unat b < LENGTH('l)\<close>
+      and \<open>sint a \<ge> 0\<close>
+      and \<open>c_signed_in_range (sint a * 2 ^ unat b) LENGTH('l)\<close>
+      and \<open>\<phi> \<longlongrightarrow> \<psi> (word_of_int (sint a * 2 ^ unat b)) \<star> \<top>\<close>
+  shows \<open>\<phi> \<longlongrightarrow> \<W>\<P> \<Gamma> (c_signed_shl a b) \<psi> \<rho> \<theta>\<close>
+proof -
+  from assms(1,2,3) have eq: \<open>c_signed_shl a b = literal (word_of_int (sint a * 2 ^ unat b))\<close>
+    by (simp add: c_signed_shl_def c_shift_out_of_range_def c_signed_overflow_def Let_def)
+  show ?thesis unfolding eq using assms(4) by (rule wp_literalI)
+qed
+
+lemma wp_c_signed_shr [micro_rust_wp_simps]:
+  fixes a b :: \<open>'l::{len} sword\<close>
+  assumes \<open>\<And>r. ucincl (\<psi> r)\<close>
+  shows \<open>\<W>\<P> \<Gamma> (c_signed_shr a b) \<psi> \<rho> \<theta> =
+    (if unat b \<ge> LENGTH('l) then \<theta> (CustomAbort ShiftOutOfRange) \<star> UNIV
+     else if sint a < 0 then \<theta> (CustomAbort SignedOverflow) \<star> UNIV
+     else \<psi> (word_of_int (sint a div 2 ^ unat b)))\<close>
+  using assms
+  by (simp add: c_signed_shr_def c_shift_out_of_range_def c_signed_overflow_def
+                c_abort_def micro_rust_wp_simps)
+
+lemma wp_c_signed_shrI [micro_rust_wp_intros]:
+  fixes a b :: \<open>'l::{len} sword\<close>
+  assumes \<open>unat b < LENGTH('l)\<close>
+      and \<open>sint a \<ge> 0\<close>
+      and \<open>\<phi> \<longlongrightarrow> \<psi> (word_of_int (sint a div 2 ^ unat b)) \<star> \<top>\<close>
+  shows \<open>\<phi> \<longlongrightarrow> \<W>\<P> \<Gamma> (c_signed_shr a b) \<psi> \<rho> \<theta>\<close>
+proof -
+  from assms(1,2) have eq: \<open>c_signed_shr a b = literal (word_of_int (sint a div 2 ^ unat b))\<close>
+    by (simp add: c_signed_shr_def c_shift_out_of_range_def c_signed_overflow_def)
+  show ?thesis unfolding eq using assms(3) by (rule wp_literalI)
+qed
+
 subsection \<open>Unsigned Division and Modulo\<close>
 
 lemma wp_c_unsigned_div [micro_rust_wp_simps]:
